Lean 4.0.0 is broken

ProveFalse.lean
@@ -1,4 +1,75 @@
-def hello := "world"
+-- Mario Carneiro found this bug.
+-- https://leanprover.zulipchat.com/#narrow/channel/270676-lean4/topic/Soundness.20bug.3A.20hasLooseBVars.20is.20not.20conservative/near/521286338
+import Lean
+open Lean
 
-theorem tt : hello = "world" := by
-  rfl
+def isProp.{u} : Prop :=
+  ∀ (x : Sort u) (y z : x), y = z
+
+theorem isProp_prop : isProp.{0} :=
+  fun _ _ _ => rfl
+
+theorem not_isProp_type : ¬ isProp.{1} :=
+  fun h => nomatch h _ 0 1
+
+theorem isProp_not_invariant : isProp.{0} ≠ isProp.{1} :=
+  mt (fun h => cast h isProp_prop) not_isProp_type
+
+def mkLevel : Nat → Level → Level
+| 0, e => e
+| Nat.succ n, e => mkLevel n (.max .zero e)
+
+open Lean Elab Command
+
+elab "add_magic" : command => do
+  let l := mkLevel (2^24) (.param `u)
+
+  liftCoreM <|
+    Lean.addDecl <|
+      Declaration.defnDecl {
+        name := `magic
+        levelParams := []
+        type := Expr.sort Level.zero
+        value := Expr.const `isProp [l]
+        hints := ReducibilityHints.opaque
+        safety := DefinitionSafety.safe
+      }
+
+add_magic
+
+elab "add_magic_eq" : command => do
+  liftCoreM do
+    Lean.addDecl <|
+      Declaration.defnDecl {
+        toConstantVal := {
+          name := `magic_eq
+          levelParams := [`u]
+          type :=
+            mkApp3
+              (mkConst ``Eq [levelOne])
+              (Expr.sort Level.zero)
+              (Expr.const `magic [])
+              (Expr.const `isProp [.param `u])
+        }
+        value :=
+          mkApp2
+            (mkConst ``Eq.refl [levelOne])
+            (Expr.sort Level.zero)
+            (Expr.const `magic [])
+        hints := ReducibilityHints.opaque
+        safety := DefinitionSafety.safe
+        all := [`magic_eq]
+      }
+
+add_magic_eq
+
+universe u
+
+example : magic = isProp.{u} :=
+  magic_eq.{u}
+
+theorem contradiction : False :=
+  isProp_not_invariant
+    (magic_eq.{0}.symm.trans magic_eq.{1})
+
+#print axioms contradiction
